ML wrapper for max_len

theories/examples/buffers.v
@@ -254,6 +254,13 @@ Section Specs.
     ∗ "HMergeInitial" ∷ (Ψframe i ∗ isBufferRecordML vbuf ℓbuf (Pb i) cap ==∗ Ψ i)
     ∗ "HCont" ∷ ▷ (Ψ (j+1)%Z -∗ Φ #()).
 
+  Definition wrap_max_len_ML s vv Φ : iProp Σ :=
+    ∃ (n:nat),
+      "->" ∷ ⌜s = wrap_max_len_name⌝
+    ∗ "->" ∷ ⌜vv = [ #n ]⌝
+    ∗ "HCont" ∷ ▷ Φ #(buffer_max_len n).
+
+
 End Specs.
 
 Section LemmasThatShouldBeInStdPP.
@@ -577,6 +584,35 @@ Section Proofs.
     wp_apply (wp_CAMLunregister1 with "[$HGC $Hℓbf]"); [done..|].
     iIntros "HGC"; wp_pure _.
     iModIntro. iApply ("Cont" with "HGC (HCont HΨ) [//] [//]").
+  Qed.
+
+
+  Lemma wrap_max_len_correct E e Ψ :
+    prims_proto E e Ψ ||- buf_lib_prog @ E :: wrap_proto (wrap_max_len_ML).
+  Proof.
+    iIntros (s ws Φ) "H". iNamed "H".
+    iNamed "Hproto".
+    cbn. unfold progwp. solve_lookup_fixed.
+    destruct lvs as [|lv [|??]]; first done.
+    all: cbn; iDestruct "Hsim" as "(->&H)"; try done.
+    destruct ws as [|w [|??]]; try (eapply Forall2_length in Hrepr; cbn in Hrepr; done).
+    eapply Forall2_cons_inv_l in Hrepr as (wcap&?&Hlval&_&?); simplify_eq.
+    cbn. iExists _. iSplit; first done.
+    iExists _. cbn. solve_lookup_fixed.
+    iSplit; first done. iNext.
+
+    wp_apply (wp_val2int with "HGC"); [done..|].
+    iIntros "HGC".
+    wp_bind (FunCall (&buffy_max_len_name) _).
+    iApply wp_proto_mono. 2: iApply wp_wand.
+    2: iApply buffy_max_len_spec.
+    1: iIntros (???) "[]".
+    1: by do 4 (apply insert_subseteq_r; [done|]).
+    1: done.
+    iIntros (v) "->".
+    wp_apply (wp_int2val with "HGC"); [done..|].
+    iIntros (w) "(HGC&%Hrepr)".
+    iApply ("Cont" with "HGC HCont [//] [//]").
   Qed.
 
 End Proofs.
